Further experiments

Forward_Hoare.thy
@@ -1,5 +1,5 @@
 theory Forward_Hoare
-  imports Main
+  imports "HOL-Library.Rewrite" "HOL-Eisbach.Eisbach" Main
   keywords "do" :: prf_decl % "proof"
 begin
 
@@ -37,13 +37,44 @@ fun postcondition1 :: "instruction \<Rightarrow> pc_spec1 \<Rightarrow> invarian
   "postcondition1 (Set x i) Trivial I = Some (\<lambda>m. m x = i \<and> (\<exists>j. I (m(x:=j))))"
 | "postcondition1 (Guess x) (Pick i) I = Some (\<lambda>m. m x = i \<and> (\<exists>j. I (m(x:=j))))"
 | "postcondition1 (Guess x) Trivial I = Some (\<lambda>m. \<exists>j. I (m(x:=j)))"
-| "postcondition1 (Add x y) Trivial I = Some (\<lambda>m. I (m(x:=m x - m y)))"
+| "postcondition1 (Add x y) Trivial I = (if x\<noteq>y then Some (\<lambda>m. I (m(x:=m x - m y))) else None)"
 | "postcondition1 _ (Pick _) _ = None"
 
 fun postcondition :: "program \<Rightarrow> pc_spec \<Rightarrow> invariant \<Rightarrow> invariant option" where
   "postcondition [] [] I = Some I"
 | "postcondition (c#p) (s#ss) I = (case postcondition1 c s I of Some I' \<Rightarrow> postcondition p ss I' | None \<Rightarrow> None)"
 | "postcondition _ _ _ = None"
+
+lemma pc_length: "postcondition p1 pc1 I \<noteq> None \<Longrightarrow> length p1 = length pc1"
+  apply (induction p1 arbitrary: I pc1)
+  using list.exhaust apply force
+  apply auto
+  apply (case_tac pc1)
+   apply auto
+  by (metis option.case_eq_if option.distinct(1))
+
+
+lemma postcondition': "postcondition (p @ [c]) (ss @ [s]) I =
+  (case postcondition p ss I of Some I' \<Rightarrow> postcondition1 c s I' | None \<Rightarrow> None)"
+proof (cases "length p = length ss")
+  case True
+  then show ?thesis
+  proof (induction arbitrary: I rule:list_induct2)
+    case Nil
+    then show ?case
+      apply (cases "postcondition1 c s I")
+      by auto
+  next
+    case (Cons x xs y ys)
+    show ?case 
+      apply (cases "postcondition1 x y I"; simp)
+      using Cons.IH by blast
+  qed
+next
+  case False
+  then show ?thesis
+    by (metis length_append_singleton nat.inject option.simps(4) pc_length)
+qed
 
 ML \<open>
 datatype pc_spec1 = Trivial | Pick of int
@@ -52,6 +83,7 @@ fun pc_spec1_to_term Trivial = \<^const>\<open>Trivial\<close>
   | pc_spec1_to_term (Pick i) = \<^const>\<open>Pick\<close> $ HOLogic.mk_number HOLogic.intT i
 fun pc_spec_to_term pc = pc |> map pc_spec1_to_term |> HOLogic.mk_list \<^typ>\<open>pc_spec1\<close>
 fun pc_spec_to_cterm ctxt pc = pc_spec_to_term pc |> Thm.cterm_of ctxt
+fun merge_pc pc1 pc2 = SOME (pc1 @ pc2)
 \<close>
 
 section \<open>Ranges\<close>
@@ -63,6 +95,9 @@ fun valid_range (program:program) ((start,endd):range) =
 (* Contract: valid_range = true *)
 fun extract_range (program:program) ((start,endd):range) : program =
   program |> drop start |> take (endd-start)
+(* Contract: valid_range = true *)
+fun merge_ranges (_:program) ((s1,e1):range) ((s2,e2):range) : range option =
+  if e1=s2 then SOME (s1,e2) else NONE
 \<close>
 
 section \<open>Joint stuff\<close>
@@ -106,20 +141,25 @@ fun make_step binding program range precondition_const postcondition lthy : loca
   fun bind suffix = Binding.suffix_name suffix binding
   val program_fragment = extract_range program range
   val program_fragment_ct = program_to_cterm lthy program_fragment
+  val _ = tracing ("Program fragment: " ^ Syntax.string_of_term lthy (Thm.term_of program_fragment_ct))
   val (program_fragment_const,lthy) = 
       def' (bind "_prog") program_fragment_ct lthy
   val postcondition_ct = pc_spec_to_cterm lthy postcondition
+  val _ = tracing ("Postcondition: " ^ Syntax.string_of_term lthy (Thm.term_of postcondition_ct))
   val (postcondition_const,lthy) = def' (bind "_pc") postcondition_ct lthy
-  val invariant_ct = \<^const>\<open>postcondition\<close> 
+  val invariant_opt_ct = \<^const>\<open>postcondition\<close> 
         $ program_fragment_const
         $ postcondition_const
-        $ precondition_const
-    |> mk_the |> Thm.cterm_of lthy
+        $ precondition_const |> Thm.cterm_of lthy
+  val _ = tracing ("Invariant: " ^ Syntax.string_of_term lthy (Thm.term_of invariant_opt_ct))
+  val (invariant_opt_const,lthy) = def' (bind "_inv_opt") invariant_opt_ct lthy
+  val invariant_ct = invariant_opt_const |> mk_the |> Thm.cterm_of lthy
   val (invariant_const,lthy) = def' (bind "_inv") invariant_ct lthy
   val spec : step_spec = {binding=binding, range=range, program_fragment=program_fragment, invariant_const=invariant_const,
     invariant_ct=invariant_ct, postcondition=postcondition, 
     postcondition_const=postcondition_const, postcondition_ct=postcondition_ct,
     program_fragment_const=program_fragment_const}
+  val _ = tracing ("Spec: " ^ \<^make_string> spec)
   val lthy = add_spec spec lthy
 in
   lthy
@@ -164,41 +204,393 @@ val _ =
     (Parse.ML_source >> (Toplevel.proof o do_cmd));
 \<close>
 
+lemma pc_impI[intro]: "(\<And>m. pc1 m \<Longrightarrow> pc2 m) \<Longrightarrow> pc_imp pc1 pc2"
+  unfolding pc_imp_def by auto
+
+lemma pc_impD[dest]: "pc_imp pc1 pc2 \<Longrightarrow> pc1 m \<Longrightarrow> pc2 m"
+  unfolding pc_imp_def by auto
+
+
+definition "independent_of (B::invariant) (x::var) = (\<forall>m1 m2. (\<forall>y\<noteq>x. m1 y = m2 y) \<longrightarrow> B m1 = B m2)"
+lemma independent_ofI: 
+  assumes "\<And>m1 m2. (\<And>y. y\<noteq>x \<Longrightarrow> m1 y = m2 y) \<Longrightarrow> B m1 = B m2"
+  shows "independent_of B x"
+  unfolding independent_of_def using assms by metis
+
+
+lemma newvalue_Guess: 
+  assumes "invariant \<equiv> the invariant_opt"
+  assumes "invariant_opt \<equiv> postcondition prog pc A"
+  assumes "prog \<equiv> [Guess x]"
+  assumes "pc \<equiv> [Pick i]"
+  shows "pc_imp invariant (\<lambda>m. m x = i)"
+  unfolding assms(1-4)
+  by (rule pc_impI; simp)
+
+lemma newvalue_Set:
+  assumes "invariant \<equiv> the invariant_opt"
+  assumes "invariant_opt \<equiv> postcondition prog pc A"
+  assumes "prog \<equiv> [Set x i]"
+  assumes "pc \<equiv> [Trivial]"
+  shows "pc_imp invariant (\<lambda>m. m x = i)"
+  unfolding assms(1-4)
+  by (rule pc_impI; simp)
+
+lemmas newvalue = newvalue_Set newvalue_Guess
+
+lemma unchanged_Guess: 
+  assumes "invariant \<equiv> the invariant_opt"
+  assumes "invariant_opt \<equiv> postcondition prog pc A"
+  assumes "prog \<equiv> [Guess x]"
+  assumes "pc \<equiv> [s]"
+  assumes indep: "independent_of B x"
+  assumes imp: "\<And>m. A m \<Longrightarrow> B m"
+  shows "pc_imp invariant B"
+  unfolding assms(1-4)
+  apply (cases s; rule pc_impI; simp)
+  using indep imp unfolding independent_of_def apply auto
+  by (metis fun_upd_def)+
+
+lemma unchanged_Add: 
+  assumes "invariant \<equiv> the invariant_opt"
+  assumes "invariant_opt \<equiv> postcondition prog pc A"
+  assumes "prog \<equiv> [Add x y]"
+  assumes "pc \<equiv> [Trivial]"
+  assumes indep: "independent_of B x"
+  assumes xy: "x \<noteq> y"
+  assumes imp: "\<And>m. A m \<Longrightarrow> B m"
+  shows "pc_imp invariant B"
+  unfolding assms(1-4)
+  apply (rule pc_impI)
+  using indep imp xy unfolding independent_of_def apply auto
+  by (metis fun_upd_def)
+
+lemma unchanged_Set: 
+  assumes "invariant \<equiv> the invariant_opt"
+  assumes "invariant_opt \<equiv> postcondition prog pc A"
+  assumes "prog \<equiv> [Set x i]"
+  assumes "pc \<equiv> [Trivial]"
+  assumes indep: "independent_of B x"
+  assumes imp: "\<And>m. A m \<Longrightarrow> B m"
+  shows "pc_imp invariant B"
+  unfolding assms(1-4)
+  apply (rule pc_impI)
+  using indep imp unfolding independent_of_def apply auto
+  by (metis fun_upd_def)
+
+lemmas unchanged = unchanged_Guess unchanged_Add unchanged_Set
+
+lemma wp_Add: 
+  assumes "invariant \<equiv> the invariant_opt"
+  assumes "invariant_opt \<equiv> postcondition prog pc A"
+  assumes "prog \<equiv> [Add x y]"
+  assumes "pc \<equiv> [Trivial]"
+  assumes distinct: "x \<noteq> y"
+  assumes imp: "\<And>m. A m \<Longrightarrow> B (m(x:=m x + m y))"
+  shows "pc_imp invariant B"
+  unfolding assms(1-4)
+  apply (rule pc_impI)
+  using distinct apply simp apply (drule imp)
+  by auto
+
+lemma wp_Set:
+  assumes "invariant \<equiv> the invariant_opt"
+  assumes "invariant_opt \<equiv> postcondition prog pc A"
+  assumes "prog \<equiv> [Set x i]"
+  assumes "pc \<equiv> [Trivial]"
+  assumes imp: "\<And>m. A m \<Longrightarrow> B (m(x:=i))"
+  shows "pc_imp invariant B"
+  unfolding assms(1-4)
+  apply (rule pc_impI)
+  apply simp
+  using imp
+  apply auto
+  apply (drule imp)
+  by auto
+
+lemmas wp = wp_Add wp_Set
+
+lemma valid_Add:
+  fixes inv
+  assumes "inv \<equiv> postcondition prog pc A"
+  assumes "prog \<equiv> [Add x y]"
+  assumes "pc \<equiv> [Trivial]"
+  assumes distinct: "x \<noteq> y"
+  shows "inv \<noteq> None"
+  unfolding assms(1-3) using distinct by simp
+
+
+lemma valid_Set:
+  fixes inv
+  assumes "inv \<equiv> postcondition prog pc A"
+  assumes "prog \<equiv> [Set x i]"
+  assumes "pc \<equiv> [Trivial]"
+  shows "inv \<noteq> None"
+  unfolding assms(1-3) by simp
+
+lemma valid_Guess:
+  fixes inv
+  assumes "inv \<equiv> postcondition prog pc A"
+  assumes "prog \<equiv> [Guess x]"
+  assumes "pc \<equiv> [s]"
+  shows "inv \<noteq> None"
+  unfolding assms(1-3) apply (cases s) by simp_all
+
+lemmas valid = valid_Set valid_Guess valid_Add
+
+ML \<open>
+fun use_facts_tac ctxt thms = 
+  EVERY' (map (fn thm => forward_tac ctxt [thm COMP @{thm pc_impD}]) (rev (tl thms)))
+  THEN' (dresolve_tac ctxt [hd thms COMP @{thm pc_impD}])
+\<close>
+
+(* method use_fact uses fact = frule fact[THEN pc_impD] *)
+
+lemma list_rev_induct2 [consumes 1, case_names Nil snoc]:
+  "length xs = length ys \<Longrightarrow> P [] [] \<Longrightarrow>
+   (\<And>x xs y ys. length xs = length ys \<Longrightarrow> P xs ys \<Longrightarrow> P (xs@[x]) (ys@[y]))
+   \<Longrightarrow> P xs ys"
+  apply (rule list_induct2[where xs="rev xs" and ys="rev ys" and P="\<lambda>xs ys. P (rev xs) (rev ys)", simplified])
+  by auto
+
+lemma pc_merge:
+  assumes "postcondition p1 pc1 I \<noteq> None"
+  shows "postcondition p2 pc2 (the (postcondition p1 pc1 I)) = postcondition (p1 @ p2) (pc1 @ pc2) I"
+  using assms
+proof (cases "length p2 = length pc2")
+  case True
+  then show ?thesis
+  proof (induction rule:list_rev_induct2)
+    case Nil
+    then show ?case
+      using assms by simp
+  next
+    case (snoc p2s p2 pc2s pc2)
+    show ?case
+      unfolding append_assoc[symmetric] postcondition'
+      by (simp add: snoc.IH)
+  qed
+next
+  case False
+  then have 1: "postcondition p2 pc2 I' = None" for I'
+    using pc_length by blast
+  from assms have "length p1 = length pc1"
+    by (rule pc_length)
+  with False have "length (p1@p2) \<noteq> length (pc1@pc2)"
+    by auto
+  then have 2: "postcondition (p1 @ p2) (pc1 @ pc2) I = None"
+    using pc_length by blast
+  from 1 2 
+  show ?thesis
+    by simp
+qed
+
+fun semantics1 :: "instruction \<Rightarrow> mem \<Rightarrow> mem set" where
+  "semantics1 (Set x i) m = {m(x:=i)}"
+| "semantics1 (Add x y) m = {m(x:=m x + m y)}"
+| "semantics1 (Guess x) m = {m(x:=i)| i. True}"
+
+fun semantics :: "program \<Rightarrow> mem \<Rightarrow> mem set" where
+  "semantics [] m = {m}"
+| "semantics (c#p) m = (\<Union>m'\<in>semantics1 c m. semantics p m')"
+
+definition hoare :: "invariant \<Rightarrow> program \<Rightarrow> invariant \<Rightarrow> bool" where
+  "hoare A p B \<longleftrightarrow> (\<forall>m. A m \<longrightarrow> (\<exists>m'\<in>semantics p m. B m'))"
+
+lemma hoare_skip[simp]: "hoare A [] A"
+  unfolding hoare_def by auto
+
+lemma hoare_cons: 
+  assumes "hoare A [c] B"
+  assumes "hoare B p C"
+  shows "hoare A (c#p) C"
+  using assms unfolding hoare_def apply auto by metis
+
+lemma hoareI1:
+  assumes "postcondition1 c s A = Some C"
+  shows "hoare A [c] C"
+proof (cases c)
+  case (Add x y)
+  show ?thesis
+    unfolding Add
+  proof (cases s)
+    case Trivial
+    show "hoare A [Add x y] C"
+      using assms 
+      unfolding hoare_def Add Trivial
+      apply auto
+      by (smt fun_upd_other fun_upd_same fun_upd_triv fun_upd_upd option.distinct(1) option.inject)
+  next
+    case (Pick i)
+    with assms Add have False
+      by simp
+    then show "hoare A [Add x y] C"
+      by simp
+  qed
+next
+  case (Set x i)
+  show ?thesis
+    unfolding Set
+  proof (cases s)
+    case Trivial
+    show "hoare A [Set x i] C"
+      using assms 
+      unfolding hoare_def Set Trivial
+      apply auto
+      by (metis fun_upd_triv)
+  next
+    case (Pick j)
+    with assms Set have False
+      by simp
+    then show "hoare A [Set x i] C"
+      by simp
+  qed
+next
+  case (Guess x)
+  show ?thesis
+    unfolding Guess
+  proof (cases s)
+    case (Pick j)
+    show "hoare A [Guess x] C"
+      using assms 
+      unfolding hoare_def Guess Pick
+      apply simp
+      by (metis (mono_tags, lifting) fun_upd_idem_iff fun_upd_same fun_upd_upd)
+  next
+    case Trivial
+    show "hoare A [Guess x] C"
+      using assms 
+      unfolding hoare_def Guess Trivial
+      apply simp
+      by (metis fun_upd_triv)
+  qed
+qed
+
+lemma hoareI0:
+  assumes "postcondition p pc A = Some B"
+  shows "hoare A p B"
+proof -
+  have "length p = length pc"
+    using assms pc_length by auto
+  from this assms show ?thesis
+  proof (induction arbitrary: A rule:list_induct2)
+    case Nil
+    then show ?case by simp
+  next
+    case (Cons c p s pc)
+    then have "postcondition (c # p) (s # pc) A = Some B"
+      by -
+    then obtain C where pc_p: "postcondition p pc C = Some B" and pc_c: "postcondition1 c s A = Some C"
+      apply (cases "postcondition1 c s A")
+      by auto
+    from pc_p have "hoare C p B"
+      using Cons.IH by auto
+    moreover from pc_c have "hoare A [c] C"
+      by (rule hoareI1)
+    ultimately show ?case
+      apply (rule_tac hoare_cons) by auto
+  qed
+qed
+
+lemma hoare_conseq:
+  assumes "pc_imp A A'"
+  assumes "pc_imp B' B"
+  assumes "hoare A' p B'"
+  shows "hoare A p B"
+  using assms unfolding hoare_def pc_imp_def by blast
+
+lemma hoareI:
+  assumes "B' \<equiv> postcondition p' pc A'"
+  assumes "B' \<noteq> None"
+  assumes AA': "pc_imp A A'"
+  assumes B'B: "pc_imp (the B') B"
+  assumes p'p: "p' = p"
+  shows "hoare A p B"
+  using AA' B'B apply (rule hoare_conseq)
+  apply (rule hoareI0)
+  using assms(1-2) unfolding p'p by auto
+
 lemma True
 proof 
 
+  define prog where "prog = [Set STR ''x'' 5, Guess STR ''y'', Add STR ''x'' STR ''y'']"
+
+  (* Step 1 *)
+
   do \<open>make_step \<^binding>\<open>step1\<close> test_prog (0,1) (#invariant_const start_spec) [Trivial]\<close>
-  have step1_exists: "postcondition step1_prog step1_pc start_inv = Some step1_inv"
-    unfolding step1_inv_def step1_prog_def step1_pc_def by simp
+
+  have step1_exists: "step1_inv_opt \<noteq> None"
+    by (rule valid, fact step1_inv_opt_def, fact step1_prog_def, fact step1_pc_def)
+
   have step1_x5: "pc_imp step1_inv (\<lambda>m. m STR ''x'' = 5)"
-    unfolding step1_inv_def pc_imp_def step1_prog_def step1_pc_def start_inv_def
-    by simp
+    by (rule newvalue, fact step1_inv_def, fact step1_inv_opt_def, fact step1_prog_def, fact step1_pc_def)
+
+  (* Step 2 *)
 
   do \<open>make_step \<^binding>\<open>step2\<close> test_prog (1,2) (#invariant_const (get_spec "step1" \<^context>)) [Pick ~5]\<close>
-  have step2_x5: "pc_imp step2_inv (\<lambda>m. m STR ''x'' = 5)"
-    using step1_x5
-    unfolding step2_prog_def step2_pc_def pc_imp_def step2_inv_def
-    by auto
-  have step2_y5: "pc_imp step2_inv (\<lambda>m. m STR ''y'' = -5)"
-    unfolding step2_inv_def step2_prog_def step2_pc_def pc_imp_def
-    by simp
-    
-  do \<open>make_step \<^binding>\<open>step3\<close> test_prog (2,3) (#invariant_const (get_spec "step2" \<^context>)) [Trivial]\<close>
-  have step3_y5: "pc_imp step3_inv (\<lambda>m. m STR ''y'' = -5)"
-    unfolding step3_inv_def
-    using step2_y5 unfolding step3_inv_def step3_prog_def step3_pc_def pc_imp_def
-    by auto
-  have step3_x0: "pc_imp step3_inv (\<lambda>m. m STR ''x'' = 0)"
-    unfolding pc_imp_def step3_inv_def step3_prog_def step3_pc_def
-  proof auto
-    fix m
-    assume s2: "step2_inv (m(STR ''x'' := m STR ''x'' - m STR ''y''))"
-    show "m STR ''x'' = 0"
-      using step2_x5[unfolded pc_imp_def, simplified, rule_format, OF s2]
-      using step2_y5[unfolded pc_imp_def, simplified, rule_format, OF s2]
-      by simp
-  qed
 
+  have step2_exists: "step2_inv_opt \<noteq> None"
+    by (rule valid, fact step2_inv_opt_def, fact step2_prog_def, fact step2_pc_def)
+
+  have step2_x5: "pc_imp step2_inv (\<lambda>m. m STR ''x'' = 5)"
+    apply (rule unchanged, fact step2_inv_def, fact step2_inv_opt_def, fact step2_prog_def, fact step2_pc_def)
+     apply (rule independent_ofI, simp)
+    apply (tactic \<open>use_facts_tac \<^context> @{thms step1_x5} 1\<close>)
+    by simp
+
+  have step2_y5: "pc_imp step2_inv (\<lambda>m. m STR ''y'' = -5)"
+    by (rule newvalue, fact step2_inv_def, fact step2_inv_opt_def, fact step2_prog_def, fact step2_pc_def)
+
+  ML_prf \<open>
+    local
+    val ctxt = \<^context>
+    val step1 = get_spec "step1" ctxt
+    val step2 = get_spec "step2" ctxt
+    in
+      val range = merge_ranges test_prog (#range step1) (#range step2) |> the
+      val pc = merge_pc (#postcondition step1) (#postcondition step2) |> the
+    end
+  \<close>
+
+  have start_step2: "step2_inv_opt = postcondition (step1_prog @ step2_prog) (step1_pc @ step2_pc) start_inv"
+    using step1_exists
+    unfolding step2_inv_opt_def step1_inv_def step1_inv_opt_def
+    by (rule pc_merge)
+
+  (* Step 3 *)
+
+  do \<open>make_step \<^binding>\<open>step3\<close> test_prog (2,3) (#invariant_const (get_spec "step2" \<^context>)) [Trivial]\<close>
+
+  have step3_exists: "step3_inv_opt \<noteq> None"
+    apply (rule valid, fact step3_inv_opt_def, fact step3_prog_def, fact step3_pc_def)
+    by simp
+
+  have step3_y5: "pc_imp step3_inv (\<lambda>m. m STR ''y'' = -5)"
+    apply (rule unchanged, fact step3_inv_def, fact step3_inv_opt_def, fact step3_prog_def, fact step3_pc_def)
+      apply (rule independent_ofI, simp)
+     apply simp
+    apply (tactic \<open>use_facts_tac \<^context> @{thms step2_y5} 1\<close>)
+    by simp
+
+  have step3_x0: "pc_imp step3_inv (\<lambda>m. m STR ''x'' = 0)"
+    apply (rule wp_Add, fact step3_inv_def, fact step3_inv_opt_def, fact step3_prog_def, fact step3_pc_def)
+     apply simp
+    apply (tactic \<open>use_facts_tac \<^context> @{thms step2_x5 step2_y5} 1\<close>)
+    by simp
+
+  have start_step3: "step3_inv_opt \<equiv> postcondition ((step1_prog @ step2_prog) @ step3_prog) ((step1_pc @ step2_pc) @ step3_pc) start_inv"
+    apply (subst pc_merge[symmetric])
+    using start_step2 step2_inv_opt_def step2_pc_def step2_prog_def apply force
+    unfolding step3_inv_opt_def step3_inv_def start_step2[symmetric] step2_inv_def
+    by simp
+
+  then have "hoare (\<lambda>_. True) prog (\<lambda>m. m STR ''x'' = 0)"
+    apply (rule hoareI)
+       apply (fact step3_exists)
+      apply (force simp: start_inv_def)
+    using step3_x0 step3_inv_def apply simp
+    unfolding step1_prog_def step2_prog_def step3_prog_def prog_def
+    by simp
 qed
 
 
